theories/Equiv/TraceEquivSimExt.v
@@ -1,0 +1,346 @@
+Require Import List.
+Require Import Util Var Val Exp Envs Map CSet AutoIndTac IL AllInRel.
+Require Import SmallStepRelations StateType StateTypeProperties.
+Require Import Sim Divergence TraceEquiv.
+
+Set Implicit Arguments.
+Unset Printing Records.
+
+Lemma sim_terminate {S1} `{StateType S1} (σ1 σ1':S1)
+      {S2} `{StateType S2} (σ2:S2) v
+: star2 step σ1 nil σ1'
+  -> normal2 step σ1'
+  -> sim bot3 SimExt σ1 σ2
+  -> result σ1' = Some v
+  -> exists σ2', star2 step σ2 nil σ2' /\ normal2 step σ2' /\ result σ2' = Some v.
+Proof.
+  intros. general induction H1.
+  - pinversion H3; subst.
+    + exfalso. eapply H2. inv H1; do 2 eexists; eauto.
+    + exfalso. eapply star2_normal in H1; eauto. subst.
+      eapply (activated_normal _ H6); eauto.
+    + eapply star2_normal in H5; eauto; subst.
+      eexists; repeat split; eauto; congruence.
+    + eapply normal_star_eq in H2; eauto. subst.
+      eexists σ2'.
+      eexists; repeat split; eauto. congruence.
+  - destruct y; isabsurd. simpl.
+    eapply IHstar2; eauto.
+    eapply sim_reduction_closed_1; eauto using star2, star2_silent.
+    Grab Existential Variables. eauto.
+Qed.
+
+Inductive prefixSpec (b:bool) {S} `{StateType S} : S -> list extevent -> Prop :=
+  | producesPrefixSpecSilent (σ:S) (σ':S) L :
+      step σ EvtTau σ'
+      -> prefixSpec b σ' L
+      -> prefixSpec b σ  L
+  | producesPrefixSpecExtern (σ:S) (σ':S) evt L :
+      activated σ
+      -> step σ evt σ'
+      -> prefixSpec b σ' L
+      -> prefixSpec b σ (EEvtExtern evt::L)
+  | producesPrefixSpecTerm (σ:S) (σ':S) r
+    : result σ' = Some r
+      -> star2 step σ nil σ'
+      -> normal2 step σ'
+      -> prefixSpec b σ (EEvtTerminate (Some r)::nil)
+  | producesPrefixSpecStuck (σ:S) (σ':S) L
+    : result σ' = None
+      -> star2 step σ nil σ'
+      -> normal2 step σ'
+      -> b
+      -> prefixSpec b σ L
+  | producesPrefixSpecPrefixSpec (σ:S)
+    : prefixSpec b σ nil.
+
+Lemma prefixSpec_star2_silent b {S} `{StateType S} (σ σ':S) L
+ : star2 step σ nil σ' ->
+   prefixSpec b σ' L -> prefixSpec b σ L.
+Proof.
+  intros. general induction H0; eauto.
+  - destruct yl, y; simpl in *; try congruence.
+    econstructor 1; eauto.
+Qed.
+
+Lemma prefixSpec_star2_silent' b {S} `{StateType S} (σ σ':S) L
+ : star2 step σ nil σ' ->
+   prefixSpec b σ L -> prefixSpec b σ' L.
+Proof.
+  intros. general induction H0; eauto.
+  - destruct yl, y; simpl in *; try congruence.
+    eapply IHstar2; eauto.
+    inv H2.
+    + relsimpl; eauto.
+    + relsimpl.
+    + exploit star2_reach_silent_step; eauto. eapply H.
+      destruct H6; subst.
+      * exfalso. eapply H5; firstorder.
+      * econstructor 3; eauto.
+    + econstructor 4; eauto. relsimpl. eauto.
+    + econstructor 5.
+Qed.
+
+Lemma bisim_prefixSpec_maintain {S} `{StateType S} {S'} `{StateType S'} (σ:S) (σ':S')
+: sim bot3 SimExt σ σ' -> forall L, prefixSpec false σ L -> prefixSpec false σ' L.
+Proof.
+  intros. general induction H2.
+  - eapply IHprefixSpec.
+    eapply sim_reduction_closed; eauto.
+    eapply star2_silent; eauto. eapply star2_refl.
+    eapply star2_refl.
+  - eapply sim_activated in H4; eauto.
+    destruct H4 as [? [? [? []]]].
+    destruct evt.
+    + edestruct H6 as [? [? ?]]; eauto.
+      eapply prefixSpec_star2_silent; eauto.
+      econstructor 2; eauto.
+    + exfalso; eapply (no_activated_tau_step _ H0 H1); eauto.
+  - eapply sim_terminate in H4; eauto.
+    destruct H4 as [? [? []]].
+    econstructor 3; [ | eauto | eauto]. congruence.
+  - isabsurd.
+  - econstructor 5.
+Qed.
+
+Lemma bisim_prefixSpec_refine {S} `{StateType S} {S'} `{StateType S'} (σ:S) (σ':S')
+: sim bot3 SimExt σ σ' -> forall L, prefixSpec true σ' L -> prefixSpec true σ L.
+Proof.
+  intros. general induction H2.
+  - eapply IHprefixSpec.
+    eapply sim_reduction_closed; eauto.
+    eapply star2_refl.
+    eapply star2_silent; eauto. eapply star2_refl.
+  - destruct evt; [|exfalso; eapply (no_activated_tau_step _ H H1); eauto].
+    eapply sim_activated_2 in H4; eauto.
+    destruct H4 as [? [? [[? [? ?]]|[? [? ?]]]]].
+    + edestruct H6 as [? [? ?]]; eauto.
+      eapply prefixSpec_star2_silent; eauto.
+      econstructor 2; eauto.
+    + econstructor 4; eauto.
+  - eapply sim_terminate_2 in H4; eauto.
+    destruct H4 as [? [? []]]. destruct H6.
+    + econstructor 3; [ | eauto | eauto]. congruence.
+    + econstructor 4; eauto.
+  - eapply sim_terminate_2 in H5; eauto.
+    destruct H5 as [? [? []]]. destruct H7.
+    + econstructor 4; eauto. congruence.
+    + econstructor 4; eauto.
+  - econstructor 5.
+Qed.
+
+
+Lemma prefixSpec_terminates S `{StateType S} (σ:S) r L
+:  prefixSpec false σ (EEvtTerminate r::L)
+   -> exists σ', star2 step σ nil σ' /\ normal2 step σ' /\ result σ' = r /\ L = nil.
+Proof.
+  intros. general induction H0.
+  - edestruct IHprefixSpec. reflexivity.
+    eexists x; dcr; subst. eauto using star2_silent.
+  - eexists; intuition; eauto.
+  - isabsurd.
+Qed.
+
+Lemma prefixSpec_nil_div S `{StateType S} σ
+  : (forall L, prefixSpec true σ L -> L = nil) -> diverges σ.
+Proof.
+  revert σ.
+  cofix f. intros.
+  destruct (@step_dec _ H σ).
+  - destruct H1; dcr. destruct x.
+    + exfalso. exploit H0. econstructor 2; try eapply H2.
+      eexists; eauto.
+      econstructor 5. congruence.
+    + econstructor. eauto. eapply f.
+      intros. eapply H0.
+      eapply prefixSpec_star2_silent.
+      eapply star2_silent; eauto. econstructor. eauto.
+  - exfalso.
+    case_eq (result σ); intros.
+    + exploit H0. econstructor 3; eauto.
+      eapply star2_refl. congruence.
+    + exploit H0. econstructor 4; eauto.
+      eapply star2_refl. instantiate (1:=EEvtTerminate None::nil) in H3.
+      congruence.
+Qed.
+
+Lemma div_prefixSpec_nil S `{StateType S} σ
+  : diverges σ -> forall L, prefixSpec true σ L -> L = nil.
+Proof.
+  intros. general induction H1; eauto.
+  - eapply IHprefixSpec.
+    eapply diverges_reduction_closed; eauto.
+    eapply star2_silent; eauto. eapply star2_refl.
+  - exfalso.
+    eapply diverges_never_activated; eauto.
+  - exfalso.
+    eapply diverges_never_terminates; eauto.
+    eapply diverges_reduction_closed; eauto.
+  - exfalso.
+    eapply diverges_never_terminates; eauto.
+    eapply diverges_reduction_closed; eauto.
+Qed.
+
+Lemma produces_diverges S `{StateType S} S' `{StateType S'} (σ:S) (σ':S')
+: (forall L, prefixSpec true σ' L -> prefixSpec true σ L)
+  -> diverges σ -> diverges σ'.
+Proof.
+  intros.
+  pose proof (div_prefixSpec_nil H2).
+  eapply prefixSpec_nil_div.
+  intros. eapply H3. eauto.
+Qed.
+
+Lemma sim_complete_diverges S `{StateType S} S' `{StateType S'} (σ:S) (σ':S') p r
+: diverges σ -> diverges σ' -> sim r p σ σ'.
+Proof.
+  revert σ σ'. pcofix COH; intros.
+  inv H2; inv H3.
+  pfold.
+  econstructor.
+  - econstructor; eauto.
+  - econstructor; eauto.
+  - right. eapply COH; eauto.
+Qed.
+
+Lemma prefixSpec_star_activated S `{StateType S} b (σ1 σ1' σ1'':S) evt L
+: star2 step σ1 nil σ1'
+  -> activated σ1'
+  -> step σ1' evt σ1''
+  -> prefixSpec b σ1'' L
+  -> prefixSpec b σ1 (EEvtExtern evt::L).
+Proof.
+  intros. general induction H0.
+  - econstructor 2; eauto.
+  - relsimpl.
+    econstructor; eauto.
+Qed.
+
+Lemma prefixSpec_extevent S `{StateType S} (σ:S) evt L
+: prefixSpec false σ (EEvtExtern evt::L)
+  -> exists σ', star2 step σ nil σ'
+          /\ activated σ'
+          /\ exists σ'', step σ' evt σ'' /\ prefixSpec false σ'' L.
+Proof.
+  intros. general induction H0.
+  - edestruct IHprefixSpec. reflexivity. dcr.
+    eexists x; split; eauto using star2_silent.
+  - eexists σ; eauto using star2.
+  - isabsurd.
+Qed.
+
+Lemma prefixSpec_extevent' S `{StateType S} (σ:S) evt L
+  : prefixSpec true σ (EEvtExtern evt::L)
+    -> activated σ
+  -> exists σ', step σ evt σ' /\ prefixSpec true σ' L.
+Proof.
+  intros.
+  inv H1; dcr.
+  inv H0; dcr.
+  - exfalso. eapply step_internally_deterministic in H3; eauto; dcr.
+    isabsurd.
+  - do 2 eexists; eauto.
+  - edestruct activated_normal_star; try eapply H1; eauto using star2.
+Qed.
+
+Lemma prefixSpec_silent_closed {S} `{StateType S}  S' `{StateType S'}
+      b (σ1 σ1':S) (σ2 σ2':S')
+: star2 step σ1 nil σ1'
+  -> star2 step σ2 nil σ2'
+  -> (forall L, prefixSpec b σ1 L -> prefixSpec b σ2 L)
+  -> (forall L, prefixSpec b σ1' L -> prefixSpec b σ2' L).
+Proof.
+  intros.
+  - eapply prefixSpec_star2_silent'; eauto. eapply H3.
+    eapply prefixSpec_star2_silent; eauto.
+Qed.
+
+Lemma prefixSpec_event_closed {S} `{StateType S}  S' `{StateType S'}
+      b (σ1 σ1':S) (σ2 σ2':S') evt
+: step σ1 evt σ1'
+  ->  step σ2 evt σ2'
+  -> (forall L, prefixSpec b σ1 L -> prefixSpec b σ2 L)
+  -> (forall L, prefixSpec b σ1' L -> prefixSpec b σ2' L).
+Proof.
+  intros Step1 Step2 EQ.
+  destruct evt.
+  - intros.
+    assert (prefixSpec b σ1 (EEvtExtern (EvtExtern call)::L)). {
+      econstructor 2. hnf; eauto 20. eauto. eauto.
+    }
+    eapply EQ in H2. inv H2.
+    + exfalso; eapply no_activated_tau_step; try eapply H3.
+      hnf; eauto 20.
+    + exploit (@step_externally_determined _ H0 _ _ _ _ Step2 H7); eauto.
+      subst. eauto.
+    + assert (activated σ2) by (hnf; eauto).
+      relsimpl.
+  - eapply prefixSpec_silent_closed; try eapply EQ;
+      eauto using star2_silent, star2.
+Qed.
+
+Lemma prefixSpec_activated {S} `{StateType S}  S' `{StateType S'}
+      b (σ1 σ1':S) (σ2 σ2':S')
+: star2 step σ1 nil σ1'
+  -> star2 step σ2 nil σ2'
+  -> (forall L, prefixSpec b σ1 L -> prefixSpec b σ2 L)
+  -> (forall L, prefixSpec b σ1' L -> prefixSpec b σ2' L).
+Proof.
+  intros.
+  - eapply prefixSpec_star2_silent'; eauto. eapply H3.
+    eapply prefixSpec_star2_silent; eauto.
+Qed.
+
+Lemma prefix_bisim S `{StateType S} S' `{StateType S'} (σ:S) (σ':S')
+  : (forall L, prefixSpec false σ L -> prefixSpec false σ' L)
+    -> (forall L, prefixSpec true σ' L -> prefixSpec true σ L)
+  -> sim bot3 SimExt σ σ'.
+Proof.
+  revert σ σ'.
+  pcofix CIH.
+  intros σ σ' LIncl UIncl.
+  destruct (three_possibilities σ) as [A|[A|A]].
+  - dcr.
+    case_eq (result x); intros.
+    + assert (prefixSpec false σ (EEvtTerminate (Some v)::nil))
+             by (econstructor 3; eauto).
+      eapply LIncl in H4.
+      eapply prefixSpec_terminates in H4. dcr.
+      pfold.
+      econstructor 4; eauto. congruence.
+    + pfold. econstructor 3; eauto.
+  - dcr. inv H3; dcr.
+    assert (prefixSpec false x1 nil) by econstructor 5.
+    assert (prefixSpec false σ (EEvtExtern (EvtExtern x0)::nil)). {
+      eapply prefixSpec_star_activated; eauto.
+    }
+    eapply LIncl in H5.
+    eapply prefixSpec_extevent in H5; dcr.
+    pose proof (prefixSpec_silent_closed H2 H7 LIncl).
+    pose proof (prefixSpec_silent_closed H7 H2 UIncl).
+    pfold. econstructor 2; eauto.
+    + intros.
+      assert (PS:prefixSpec false x (EEvtExtern evt::nil)). {
+        eapply prefixSpec_star_activated; eauto using star2, prefixSpec.
+      }
+      eapply H5 in PS.
+      eapply prefixSpec_extevent in PS; dcr.
+      relsimpl.
+      eexists; split. eauto.
+      right. eapply CIH.
+      eapply prefixSpec_event_closed; eauto.
+      eapply prefixSpec_event_closed; eauto.
+    + intros.
+      assert (PS:prefixSpec true x2 (EEvtExtern evt::nil)). {
+        eapply prefixSpec_star_activated; eauto using star2, prefixSpec.
+      }
+      eapply H8 in PS.
+      eapply prefixSpec_extevent' in PS; dcr; eauto.
+      eexists; split. eauto.
+      right. eapply CIH.
+      eapply prefixSpec_event_closed; eauto.
+      eapply prefixSpec_event_closed; eauto.
+  - assert (diverges σ').
+    eapply (produces_diverges UIncl); eauto.
+    eapply sim_complete_diverges; eauto.
+Qed.
